simulation/correct_get_offset.v
@@ -1,0 +1,77 @@
+From bpf.comm Require Import Regs State Monad.
+From bpf.monadicmodel Require Import rBPFInterpreter.
+From Coq Require Import List Lia ZArith.
+From compcert Require Import Integers Values Clight Memory.
+Import ListNotations.
+
+From bpf.proof Require Import Clightlogic MatchState CorrectRel CommonLemma.
+
+From bpf.clight Require Import interpreter.
+
+
+(**
+Check get_offset.
+get_offset
+     : int64 -> M int
+
+ *)
+
+Open Scope Z_scope.
+
+Section Get_offset.
+
+  (** The program contains our function of interest [fn] *)
+  Definition p : Clight.program := prog.
+
+  (* [Args,Res] provides the mapping between the Coq and the C types *)
+  (* Definition Args : list CompilableType := [stateCompilableType].*)
+  Definition args : list Type := [(int64:Type)].
+  Definition res : Type := (int:Type).
+
+  (* [f] is a Coq Monadic function with the right type *)
+  Definition f : arrow_type args (M res) := get_offset.
+
+  (* [fn] is the Cligth function which has the same behaviour as [f] *)
+  Definition fn: Clight.function := f_get_offset.
+
+  (* [match_arg] relates the Coq arguments and the C arguments *)
+  Definition match_arg_list : DList.t (fun x => x -> val -> State.state -> Memory.Mem.mem -> Prop) args :=
+    (DList.DCons (stateless int64_correct)
+                    (DList.DNil _)).
+
+  (* [match_res] relates the Coq result and the C result *)
+  Definition match_res : res -> val -> State.state -> Memory.Mem.mem -> Prop := fun x v st m => sint32_correct x v.
+
+  Instance correct_function3_get_offset : forall a, correct_function3 p args res f fn (nil) true match_arg_list match_res a.
+  Proof.
+    correct_function_from_body args.
+    correct_body.
+    (** how to use correct_* *)
+    unfold INV.
+    unfold f.
+    repeat intro.
+    get_invariant _ins.
+
+    unfold stateless, int64_correct in c0.
+    subst.
+
+    eexists; exists m, Events.E0.
+
+    split.
+    {
+      forward_star.
+      forward_star.
+    }
+    split.
+    {
+      unfold match_res, sint32_correct, Regs.get_offset; simpl.
+      (**r according to the clight representation, we delete the self-defined library int16 in order to simplify the proof here *)
+      reflexivity.
+    }
+    split;[constructor; reflexivity | split; reflexivity].
+  Qed.
+
+End Get_offset.
+Close Scope Z_scope.
+
+Existing Instance correct_function3_get_offset.
