src/DxAST.v
@@ -11,22 +11,6 @@ From dx.Type Require Import Bool Nat.
 From bpf.comm Require Import rBPFAST.
 From bpf.src Require Import CoqIntegers DxIntegers DxValues.
 
-(*
-Definition well_chunk_Z (chunk: memory_chunk):Z := 
-  match chunk with
-  | Mint8unsigned => 1
-  | Mint16unsigned => 2
-  | Mint32 => 4
-  | Mint64 => 8
-  | _ => 10
-  end.
-
-Definition memory_chunk_to_valu32 (chunk: memory_chunk): valu32_t := 
-  Vint (Int.repr (well_chunk_Z chunk)). (**r well_chunk implies align_chunk, so we didn't need align_chunk, but we must prove a lemma! *)
-
-Definition memory_chunk_to_valu32_upbound (chunk: memory_chunk): valu32_t :=
-  Vint (Int.repr (Int.max_unsigned-(well_chunk_Z chunk))).
-*)
 (******************** Dx Related *******************)
 
 Definition memoryChunkCompilableType :=
