src/DxRegs.v
@@ -11,255 +11,6 @@ From bpf.src Require Import IdentDef CoqIntegers DxIntegers DxValues. (* GenMatc
 From Coq Require Import List ZArith.
 Import ListNotations.
 
-(*
-Inductive reg: Type :=
-  | R0:reg | R1:reg | R2:reg
-  | R3:reg | R4:reg | R5:reg
-  | R6:reg | R7:reg | R8:reg
-  | R9:reg | R10:reg
-.
-
-Lemma reg_eq: forall (x y: reg), {x=y} + {x<>y}.
-Proof.
-decide equality. Defined.
-
-Record regmap: Type := make_regmap{
-  r0_val  : Values.val;
-  r1_val  : Values.val;
-  r2_val  : Values.val;
-  r3_val  : Values.val;
-  r4_val  : Values.val;
-  r5_val  : Values.val;
-  r6_val  : Values.val;
-  r7_val  : Values.val;
-  r8_val  : Values.val;
-  r9_val  : Values.val;
-  r10_val : Values.val;
-}.
-
-Definition eval_regmap (r:reg) (regs:regmap): val64_t := 
-  match r with
-  | R0  => r0_val regs
-  | R1  => r1_val regs
-  | R2  => r2_val regs
-  | R3  => r3_val regs
-  | R4  => r4_val regs
-  | R5  => r5_val regs
-  | R6  => r6_val regs
-  | R7  => r7_val regs
-  | R8  => r8_val regs
-  | R9  => r9_val regs
-  | R10 => r10_val regs
-  end.
-
-Definition upd_regmap (r:reg) (v:val64_t) (regs:regmap): regmap :=
-  match r with
-  | R0  => 
-    {|
-      r0_val  := v;
-      r1_val  := r1_val regs;
-      r2_val  := r2_val regs;
-      r3_val  := r3_val regs;
-      r4_val  := r4_val regs;
-      r5_val  := r5_val regs;
-      r6_val  := r6_val regs;
-      r7_val  := r7_val regs;
-      r8_val  := r8_val regs;
-      r9_val  := r9_val regs;
-      r10_val := r10_val regs;
-    |} 
-  | R1  => 
-    {|
-      r0_val  := r0_val regs;
-      r1_val  := v;
-      r2_val  := r2_val regs;
-      r3_val  := r3_val regs;
-      r4_val  := r4_val regs;
-      r5_val  := r5_val regs;
-      r6_val  := r6_val regs;
-      r7_val  := r7_val regs;
-      r8_val  := r8_val regs;
-      r9_val  := r9_val regs;
-      r10_val := r10_val regs;
-    |}
-  | R2  => 
-    {|
-      r0_val  := r0_val regs;
-      r1_val  := r1_val regs;
-      r2_val  := v;
-      r3_val  := r3_val regs;
-      r4_val  := r4_val regs;
-      r5_val  := r5_val regs;
-      r6_val  := r6_val regs;
-      r7_val  := r7_val regs;
-      r8_val  := r8_val regs;
-      r9_val  := r9_val regs;
-      r10_val := r10_val regs;
-    |} 
-  | R3  => 
-    {|
-      r0_val  := r0_val regs;
-      r1_val  := r1_val regs;
-      r2_val  := r2_val regs;
-      r3_val  := v;
-      r4_val  := r4_val regs;
-      r5_val  := r5_val regs;
-      r6_val  := r6_val regs;
-      r7_val  := r7_val regs;
-      r8_val  := r8_val regs;
-      r9_val  := r9_val regs;
-      r10_val := r10_val regs;
-    |} 
-  | R4  => 
-    {|
-      r0_val  := r0_val regs;
-      r1_val  := r1_val regs;
-      r2_val  := r2_val regs;
-      r3_val  := r3_val regs;
-      r4_val  := v;
-      r5_val  := r5_val regs;
-      r6_val  := r6_val regs;
-      r7_val  := r7_val regs;
-      r8_val  := r8_val regs;
-      r9_val  := r9_val regs;
-      r10_val := r10_val regs;
-    |} 
-  | R5  => 
-    {|
-      r0_val  := r0_val regs;
-      r1_val  := r1_val regs;
-      r2_val  := r2_val regs;
-      r3_val  := r3_val regs;
-      r4_val  := r4_val regs;
-      r5_val  := v;
-      r6_val  := r6_val regs;
-      r7_val  := r7_val regs;
-      r8_val  := r8_val regs;
-      r9_val  := r9_val regs;
-      r10_val := r10_val regs;
-    |} 
-  | R6  => 
-    {|
-      r0_val  := r0_val regs;
-      r1_val  := r1_val regs;
-      r2_val  := r2_val regs;
-      r3_val  := r3_val regs;
-      r4_val  := r4_val regs;
-      r5_val  := r5_val regs;
-      r6_val  := v;
-      r7_val  := r7_val regs;
-      r8_val  := r8_val regs;
-      r9_val  := r9_val regs;
-      r10_val := r10_val regs;
-    |} 
-  | R7  => 
-    {|
-      r0_val  := r0_val regs;
-      r1_val  := r1_val regs;
-      r2_val  := r2_val regs;
-      r3_val  := r3_val regs;
-      r4_val  := r4_val regs;
-      r5_val  := r5_val regs;
-      r6_val  := r6_val regs;
-      r7_val  := v;
-      r8_val  := r8_val regs;
-      r9_val  := r9_val regs;
-      r10_val := r10_val regs;
-    |} 
-  | R8  => 
-    {|
-      r0_val  := r0_val regs;
-      r1_val  := r1_val regs;
-      r2_val  := r2_val regs;
-      r3_val  := r3_val regs;
-      r4_val  := r4_val regs;
-      r5_val  := r5_val regs;
-      r6_val  := r6_val regs;
-      r7_val  := r7_val regs;
-      r8_val  := v;
-      r9_val  := r9_val regs;
-      r10_val := r10_val regs;
-    |} 
-  | R9  => 
-    {|
-      r0_val  := r0_val regs;
-      r1_val  := r1_val regs;
-      r2_val  := r2_val regs;
-      r3_val  := r3_val regs;
-      r4_val  := r4_val regs;
-      r5_val  := r5_val regs;
-      r6_val  := r6_val regs;
-      r7_val  := r7_val regs;
-      r8_val  := r8_val regs;
-      r9_val  := v;
-      r10_val := r10_val regs;
-    |} 
-  | R10 => 
-    {|
-      r0_val  := r0_val regs;
-      r1_val  := r1_val regs;
-      r2_val  := r2_val regs;
-      r3_val  := r3_val regs;
-      r4_val  := r4_val regs;
-      r5_val  := r5_val regs;
-      r6_val  := r6_val regs;
-      r7_val  := r7_val regs;
-      r8_val  := r8_val regs;
-      r9_val  := r9_val regs;
-      r10_val := v;
-    |} 
-  end.
-
-Definition init_regmap: regmap := {|
-  r0_val  := val64_zero;
-  r1_val  := val64_zero;
-  r2_val  := val64_zero;
-  r3_val  := val64_zero;
-  r4_val  := val64_zero;
-  r5_val  := val64_zero;
-  r6_val  := val64_zero;
-  r7_val  := val64_zero;
-  r8_val  := val64_zero;
-  r9_val  := val64_zero;
-  r10_val := val64_zero;
-|}.
-
-Open Scope Z_scope.
-
-Definition z_to_reg (z:Z): reg :=
-  if (Z.eqb z 0) then
-    R0
-  else if (Z.eqb z 1) then
-    R1
-  else if (Z.eqb z 2) then
-    R2
-  else if (Z.eqb z 3) then
-    R3
-  else if (Z.eqb z 4) then
-    R4
-  else if (Z.eqb z 5) then
-    R5
-  else if (Z.eqb z 6) then
-    R6
-  else if (Z.eqb z 7) then
-    R7
-  else if (Z.eqb z 8) then
-    R8
-  else if (Z.eqb z 9) then
-    R9
-  else
-    R10.
-
-Definition get_dst (i:int64_t):Z := Int64.unsigned (Int64.shru (Int64.and i int64_0xfff) int64_8).
-Definition get_src (i:int64_t):Z := Int64.unsigned (Int64.shru (Int64.and i int64_0xffff) int64_12).
-
-Definition int64_to_dst_reg (ins: int64_t): reg :=
-  z_to_reg (get_dst ins).
-
-Definition int64_to_src_reg (ins: int64_t): reg :=
-  z_to_reg (get_src ins).
-*)
-
 (******************** Dx Related *******************)
 
 (** Coq2C: reg -> unsigned int;
@@ -319,6 +70,22 @@ Definition Const_int64_to_src_reg :=
                            | _       => Err PrimitiveEncodingFailed
                            end).
 
+Definition Const_int64_to_offset :=
+  MkPrimitive int64Tosint32SymbolType
+                get_offset
+                (fun es => match es with
+                           | [e1] => Ok (Csyntax.Ecast (Csyntax.Ecast (Csyntax.Ebinop Cop.Oshr (Csyntax.Ebinop Cop.Oshl e1 C_U64_32 C_U64) C_U64_48 C_U64) C_S16) C_S32)
+                           | _       => Err PrimitiveEncodingFailed
+                           end).
+
+Definition Const_int64_to_immediate :=
+  MkPrimitive int64Tosint32SymbolType
+                get_immediate
+                (fun es => match es with
+                           | [e1] => Ok (Csyntax.Ecast (Csyntax.Ebinop Cop.Oshr e1 C_U64_32 C_U64) C_S32)
+                           | _       => Err PrimitiveEncodingFailed
+                           end).
+
 
 (** Coq2C: regmap -> unsigned long long int regmap[11];
   *)
@@ -356,6 +123,8 @@ Definition Const_upd_regmap :=
                            | _       => Err PrimitiveEncodingFailed
                            end).
 
+
+
 Module Exports.
   Definition regCompilableType      := regCompilableType.
   Definition Const_R0               := Const_R0.
@@ -371,6 +140,8 @@ Module Exports.
   Definition Const_R10              := Const_R10.
   Definition Const_int64_to_dst_reg := Const_int64_to_dst_reg.
   Definition Const_int64_to_src_reg := Const_int64_to_src_reg.
+  Definition Const_int64_to_offset  := Const_int64_to_offset.
+  Definition Const_int64_to_immediate := Const_int64_to_immediate.
   Definition regmapCompilableType   := regmapCompilableType.
   Definition Const_eval_regmap      := Const_eval_regmap.
   Definition Const_upd_regmap       := Const_upd_regmap.
