src/Tests.v
@@ -10,7 +10,7 @@ From compcert.lib Require Import Integers.
 From dx Require Import ResultMonad IR CoqIR IRtoC DXModule DumpAsC.
 From dx.Type Require Bool Nat.
 
-From bpf.comm Require Import Int16 MemRegion rBPFValues rBPFAST rBPFMemType Flag Regs.
+From bpf.comm Require Import MemRegion rBPFValues rBPFAST rBPFMemType Flag Regs.
 From bpf.src Require Import DxIntegers DxList64 DxValues DxRegs DxState DxOpcode DxFlag DxInstructions DxAST DxMemRegion DxMemType DxMonad DxNat.
 
 (***************************************)
