Makefile
@@ -44,7 +44,7 @@ COQEMONADIC =  $(addprefix monadicmodel/, Opcode.v rBPFInterpreter.v)
 COQSRC =  $(addprefix src/, InfComp.v GenMatchable.v CoqIntegers.v DxIntegers.v DxValues.v DxNat.v DxAST.v DxFlag.v DxList64.v DxOpcode.v IdentDef.v DxMemType.v DxMemRegion.v DxRegs.v DxState.v DxMonad.v DxInstructions.v Tests.v TestMain.v ExtrMain.v)
 COQEQUIV =  $(addprefix equivalence/, switch.v equivalence1.v equivalence2.v)
 COQISOLATION = $(addprefix isolation/, CommonISOLib.v AlignChunk.v RegsInv.v MemInv.v IsolationLemma.v Isolation.v)
-COQCOMM = $(addprefix comm/, Flag.v Int16.v LemmaNat.v List64.v rBPFAST.v rBPFMemType.v rBPFValues.v MemRegion.v Regs.v State.v Monad.v)
+COQCOMM = $(addprefix comm/, Flag.v LemmaNat.v List64.v rBPFAST.v rBPFMemType.v rBPFValues.v MemRegion.v Regs.v State.v Monad.v)
 
 #COQCOMM = $(wildcard comm/*.v)
 #COQMODEL = $(wildcard model/*.v)
@@ -124,9 +124,9 @@ clightmodel:
 	$(COQMAKEFILE) -f _CoqProject clight/interpreter.v COQEXTRAFLAGS = '-w all,-extraction'  -o CoqMakefile
 	make -f CoqMakefile
 
-PROOF = $(addprefix simulation/, correct_upd_pc.v correct_eval_pc.v correct_upd_pc_incr.v correct_eval_reg.v  correct_eval_flag.v correct_upd_flag.v correct_eval_mrs_regions.v correct_get_addr_ofs.v correct_get_dst.v correct_get_immediate.v correct_is_well_chunk_bool.v correct_get_block_ptr.v correct_get_block_size.v correct_get_start_addr.v correct_get_block_perm.v correct_get_add.v correct_get_sub.v correct_upd_reg.v correct_reg64_to_reg32.v correct_get_opcode_alu64.v correct_get_opcode_branch.v correct_step_opcode_alu64.v correct_step_opcode_branch.v correct_check_mem_aux2.v correct_get_mem_region.v correct_eval_ins_len.v correct_eval_ins.v)
+PROOF = $(addprefix simulation/, correct_upd_pc.v correct_eval_pc.v correct_upd_pc_incr.v correct_eval_reg.v  correct_eval_flag.v correct_upd_flag.v correct_eval_mrs_regions.v correct_get_addr_ofs.v correct_get_dst.v correct_get_immediate.v correct_is_well_chunk_bool.v correct_get_block_ptr.v correct_get_block_size.v correct_get_start_addr.v correct_get_block_perm.v correct_get_add.v correct_get_sub.v correct_upd_reg.v correct_reg64_to_reg32.v correct_get_opcode_alu64.v correct_get_opcode_alu32.v correct_get_opcode_branch.v correct_step_opcode_alu64.v correct_step_opcode_branch.v correct_check_mem_aux2.v correct_get_mem_region.v correct_eval_ins_len.v correct_eval_ins.v correct_eval_immediate.v correct_get_offset.v)
 
-# correct_check_mem_aux.v  correct_load_mem.v correct_get_offset.v correct_eval_immediate.v etc
+# correct_check_mem_aux.v  correct_load_mem.v etc
 
 CLIGHTLOGICDIR =  $(addprefix proof/, clight_exec.v CommonLib.v Clightlogic.v MatchState.v CorrectRel.v CommonLemma.v CommonLemmaNat.v)
 
